---
title: "ëª‡ëª‡ ì¦ëª…ë“¤"
number-sections: true
number-depth: 3
crossref:
  chapters: true
---


::: {#prp-part3_exponent_of_operator_1}

íë² ë¥´íŠ¸ ê³µê°„ $\mathscr{H}$ ì—ì„œ ì •ì˜ëœ ì—°ì‚°ì $M,\, N$ ì— ëŒ€í•´ ë‹¤ìŒ $[M,\,N]=0$ ì´ë©´ $e^{M+N} =e^M e^N$ ì´ë‹¤.

:::


::: {.proof}

::: {.callout-tip appearance="minimal"}

[MathExchange ì˜ ì§ˆë¬¸ê³¼ ë‹µë³€](https://math.stackexchange.com/questions/568450/m-n-in-bbb-r-n-times-n-show-that-emn-emen-given-mn-nm) ê°€ìš´ë° Robert Lewis ì˜ ì¦ëª…ì„ ìš”ì•½í•œë‹¤.
:::

í–‰ë ¬ì— ëŒ€í•œ ë‹¤ìŒ ìƒë¯¸ë¶„ ë°©ì •ì‹ê³¼ ì´ˆê¸°ì¡°ê±´ì´ ì£¼ì–´ì ¸ ìˆë‹¤ê³  í•˜ì.

$$
dX/dt=(M+N)X \qquad \text{with }X(0)=I
$$ {#eq-exp_op_1}

ì´ ë¯¸ë¶„ë°©ì •ì‹ì— ëŒ€í•œ ìœ ì¼í•´ëŠ” ë‹¤ìŒê³¼ ê°™ë‹¤.

$$
X(t)=e^{(ğ‘€+ğ‘)ğ‘¡}
$$ {#eq-exp_op_2}

ì´ë‹¤. ì´ì œ

$$
Y(t)=e^{Mt}e^{Nt}
$${#eq-exp_op_3}

ë¼ê³  í•˜ì. ê·¸ë ‡ë‹¤ë©´ 
$$
dY/dt=\dfrac{d(e^{ğ‘€ğ‘¡})}{dt} e^{Nt} + e^{Mt}\dfrac{d(e^{Nt})}{dt}= Me^{Mt}e^{Nt} + e^{Mt}Ne^{Nt}
$${#eq-exp_op_4}

ì´ë‹¤. $[M,\,N]= MN-NM=0$ ì´ë¯€ë¡œ $[e^{Mt},\, N]=0$ ì´ë©° ë”°ë¼ì„œ

$$
\dfrac{dY}{dt} = Me^{Mt} e^{Nt} + Ne^{Mt}e^{Nt} = (M+N)Y
$$

ì´ê³ 

$$
Y(0)=I
$$

ì´ë‹¤. $X(t)$ ì™€ $Y(t)$ ê°€ ê°™ì€ ë¯¸ë¶„ë°©ì •ì‹ê³¼ ê°™ì€ ì´ˆê¸°ì¡°ê±´ì„ ê°€ì§€ë¯€ë¡œ $X(t)=Y(t)$ ì´ë©°, ë”°ë¼ì„œ

$$
e^{(M+N)t} = e^{Mt} e^{Nt}
$$

ì´ë‹¤. $t=1$ ì—ì„œ ì„±ë¦½í•˜ë©° ì´ëŠ” ì£¼ì–´ì§„ ì‹ì´ë‹¤. $\square$


:::

</br>

::: {#prp-part3_Baker_Hausdorff_Lemma}

#### Baker-Hausdorff Lemma

$\lambda$ ê°€ ì‹¤ìˆ˜ì¼ ë•Œ ë‹¤ìŒì´ ì„±ë¦½í•œë‹¤.
$$
e^{iG\lambda}Ae^{-iG\lambda} = A + i\lambda [G,\,A] + \dfrac{(i\lambda)^2}{2!} [G,\,[G,\,A]] + \cdots + \dfrac{(i\lambda)^n}{n!} \underbrace{[G,\,[G,\,[G,\cdots [G}_{n\text{ times}},\,A]]]] + \cdots 
$$

:::

::: {.proof}

::: {.callout-tip appearance="minimal"}

[MathExchange ì˜ ì§ˆë¬¸ê³¼ ë‹µë³€](https://math.stackexchange.com/questions/711308/baker-hausdorff-lemma-from-sakurais-book) ê°€ìš´ë° Robert Lewis ì˜ ì¦ëª…ì„ ìš”ì•½í•œë‹¤.
:::

$A,\,B$ ê°€ íë² ë¥´íŠ¸ ê³µê°„ $\mathcal{H}$ ì—ì„œ ì •ì˜ëœ ì—°ì‚°ìë¼ê³  í•˜ì. ì—ë¥´ë¯¸íŠ¸ì—¬ë¶€ëŠ” ìƒê´€ ì—†ë‹¤. ì„ í˜•ì—°ì‚°ìì— ëŒ€í•œ ìƒë¯¸ë¶„ ë°©ì •ì‹

$$
\dfrac{dX}{d\lambda} = [B,\,X]
$$ {#eq-baker_1}

ê°€ ì´ˆê¸°ì¡°ê±´ $X(0)=A$ ë¥¼ ë§Œì¡±í•œë‹¤ê³  í•˜ì. ê·¸ë ‡ë‹¤ë©´

$$
X(\lambda) = e^{\lambda B}Ae^{-\lambda B}
$$ {#eq-baker_2}

ëŠ” ì´ ë¯¸ë¶„ë°©ì •ì‹ì˜ í•´ë¼ëŠ” ê²ƒì„ ë³´ì¼ ìˆ˜ ìˆë‹¤.

$$
\begin{aligned}
\dfrac{dX}{d\lambda} = Be^{\lambda B} A e^{-\lambda B} - e^{\lambda B} A e^{-\lambda B}B = [B,\,X]
\end{aligned}
$${#eq-baker_3}

ì´ë©° $X(0)=A$ ì´ê¸° ë•Œë¬¸ì´ë‹¤.

ì„ì˜ì˜ $B\in \mathcal{L}(\mathscr{H})$ ì— ëŒ€í•´ $\phi_B:\mathcal{L}(\mathscr{H}) \to \mathcal{L}(\mathscr{H})$ ë¥¼ ë‹¤ìŒê³¼ ê°™ì´ ì •ì˜í•˜ì.

$$
\phi_B(A) = [B,\, A]
$$ {#eq-baker_4}

ì—°ì‚°ì ë…¸ë¦„ $\| \cdot \|$ ì— ëŒ€í•´

$$
\begin{aligned}
\|\phi_B(A)\| &= \|[B,\,A]\| = \|BA-AB\| \\
& \le \|BA-AB\| \le \|B\|\|A\| + \|A\|\|B\| = 2\|A\|\|B\|
\end{aligned}
$$

ê°€ ì„±ë¦½í•œë‹¤. ì¦‰ $\|\phi_B\| \le 2\|B\|$ ì´ë‹¤. ì´ëŠ” $e^{\lambda B}$ ê°€ ì •ì˜ëœë‹¤ë©´ $e^{\lambda \phi_B}$ ë„ ì •ì˜ëœë‹¤ëŠ” ì˜ë¯¸ì´ë‹¤.

ë˜í•œ,

$$
\begin{aligned}
\phi_B^2(A) &= \phi_B([B,\,A]) = [B,\,[B,\,A]], \\
\phi_B^3(A) &= [B,\, [B,\,[B,\,A]]]
\end{aligned}
$$

ì´ê³  ë‹¤ìŒì„ ì‰½ê²Œ ë³´ì¼ ìˆ˜ ìˆë‹¤.

$$
{\phi_B}^n (A) = \underbrace{[B,\,[B,\,[B,\cdots [B}_{n\text{ times}},\,A]]]].
$$

ì´ì œ $Y(\lambda)$ ë¥¼ ì •í•´ì§„ $A,\,B$ ì— ëŒ€í•´ ë‹¤ìŒê³¼ ê°™ì´ ì •ì˜í•˜ì.

$$
Y(\lambda) = A+\lambda [B,\,A] + \dfrac{\lambda^2}{2!}[B,\,[B,\,A]] + \cdots + \dfrac{\lambda^n}{n!}\underbrace{[B,\,[B,\,[B,\cdots [B}_{n\text{ times}},\,A]]]] + \cdots 
$$

$\phi_B$ ë¥¼ ì´ìš©í•˜ì—¬

$$
Y(\lambda) = \sum_{n=0}^\infty \dfrac{\lambda^n}{n!} {\phi_B}^n (A) = e^{\lambda \phi_B(A)}
$$

ì„ì„ ë³´ì¼ ìˆ˜ ìˆë‹¤. ì´ $Y(\lambda)$ ì— ëŒ€í•´

$$
\dfrac{dY}{d\lambda} = \phi_B(e^{\lambda \phi_B(A)}) = [B,\, Y]
$$

ì´ë©° $Y(0) = A$ ì„ì„ ë³´ì¼ ìˆ˜ ìˆë‹¤. ì¦‰ $Y(\lambda) = X(\lambda)$ ì´ë‹¤. 


Let ğ´ and ğµ be any two operators on the Hilbert space â„‹, hermitian or not. We assume ğ´,ğµâˆˆğ¿(â„‹), the Banach algebra of bounded linear maps from â„‹ to itself. Consider the linear operator ordinary differential equation

ğ‘‘ğ‘‹ğ‘‘ğœ†=[ğµ,ğ‘‹](1)

with initial condition

ğ‘‹(0)=ğ´.(2)

We observe that

ğ‘‹(ğœ†)=ğ‘’ğœ†ğµğ´ğ‘’âˆ’ğœ†ğµ(3)

is the unique solution to (1), (2), for from (3) it follows that

ğ‘‘ğ‘‹ğ‘‘ğœ†=ğ‘’ğœ†ğµğ‘‘ğœ†ğ´ğ‘’âˆ’ğœ†ğµ+ğ‘’ğœ†ğµğ‘‘ğ´ğ‘‘ğœ†ğ‘’âˆ’ğœ†ğµ+ğ‘’ğœ†ğµğ´ğ‘’âˆ’ğœ†ğµğ‘‘ğœ†= ğµğ‘’ğœ†ğµğ´ğ‘’âˆ’ğœ†ğµâˆ’ğ‘’ğœ†ğµğ´ğ‘’âˆ’ğœ†ğµğµ=[ğµ,ğ‘’ğœ†ğµğ´ğ‘’âˆ’ğœ†ğµ],(4)

where we have used the fact that ğ‘‘ğ´/ğ‘‘ğœ†=0 and the Leibniz product rule for derivatives in (4), and furthermore it is evident from (3) that ğ‘‹(0)=ğ´.

We next recall that for any ğµâˆˆğ¿(â„‹) the adjoint linear operator adğµ:ğ¿(â„‹)â†’ğ¿(â„‹) may be defined via

adğµ(ğ´)=[ğµ,ğ´](5)

for all ğ´âˆˆğ¿(â„‹). Denoting by â€–ğ‘‡â€–ğ¿ the standard operator norm on ğ¿(â„‹), we see that

â€–adğµ(ğ´)â€–ğ¿=â€–[ğµ,ğ´]â€–ğ¿=â€–ğµğ´âˆ’ğ´ğµâ€–ğ¿â‰¤â€–ğµğ´â€–ğ¿+â€–ğ´ğµâ€–ğ¿ â‰¤â€–ğµâ€–ğ¿â€–ğ´â€–ğ¿+â€–ğ´â€–ğ¿â€–ğµâ€–ğ¿=2â€–ğµâ€–ğ¿â€–ğ´â€–ğ¿,(6)

which shows that

â€–adğµâ€–ğ¿â‰¤2â€–ğµâ€–ğ¿,(7)

i.e. that adğµâˆˆğ¿(â„‹) is itself a bounded linear operator of norm at most 2â€–ğµâ€–ğ¿. Furthermore, we have

ad2ğµ(ğ´)=adğµ(adğµ(ğ´))=adğµ([ğµ,ğ´])=[ğµ,[ğµ,ğ´]],(8)

ad3ğµ(ğ´)=adğµ(ad2ğµ(ğ´))=adğµ([ğµ,[ğµ,ğ´]])=[ğµ,[ğµ,[ğµ,ğ´]]],(9)

and so on:

adğ‘›ğµ(ğ´)=[ğµ,[ğµ,[ğµ,...[ğµ,ğ´]]]...],(10)

where the operator adğµ=[ğµ,â‹…] occurs a total of ğ‘› times on the right-hand side of (10). We see that in fact (1) may be written in terms of adğµ as

ğ‘‘ğ‘‹ğ‘‘ğœ†=adğµ(ğ‘‹).(11)

Now set

ğ‘Œ(ğœ†)=ğ´+ğœ†[ğµ,ğ´]+ğœ†22![ğµ,[ğµ,ğ´]] +â€¦+ğœ†ğ‘›ğ‘›![ğµ,[ğµ,[ğµ,â€¦[ğµî„½î„¾î…î…‹î…‹î…‹î…‹î…‹î…‹ğ‘›times,ğ´]]]]â€¦]+â€¦;(12)

from the above we see that ğ‘Œ(ğœ†) may be written

ğ‘Œ(ğœ†)=ğ´+ğœ†adğµ(ğ´)+ğœ†22!ad2ğµ(ğ´)+â€¦+ğœ†ğ‘›ğ‘›!adğ‘›ğµ(ğ´)+â€¦ =âˆ‘âˆ0ğœ†ğ‘›ğ‘›!adğ‘›ğµ(ğ´)+â€¦=ğ‘’ğœ†adğµ(ğ´);(13)

since by (7) adğµ is a bounded operator on ğ¿(â„‹), all the series occuring above converge absolutely and uniformly on compacta for all ğœ†âˆˆâ„, in fact for all ğœ†âˆˆâ„‚. We thus have, exactly as in the case of ordinary calculus, that the derivative ğ‘Œâ€²(ğœ†) is given by

ğ‘‘ğ‘Œğ‘‘ğœ†=adğµ(ğ‘’ğœ†adğµ(ğ´))=[ğµ,ğ‘’ğœ†adğµ(ğ´)],(14)

and furthermore

ğ‘Œ(0)=ğ´,(15)

which follows trivially from (12) and/or (13). Comparing (1), (2), (11), (14) and (15), we see that ğ‘‹(ğœ†) and ğ‘Œ(ğœ†), satisfying as they do the same ODE with identical initial conditions, must by uniqueness etc. be identical for all ğœ†: ğ‘‹(ğœ†)=ğ‘Œ(ğœ†). Using (3) and (12), (13) we thus see that

ğ‘’ğœ†ğµğ´ğ‘’âˆ’ğœ†ğµ=ğ‘’ğœ†adğµ(ğ´) =ğ´+ğœ†[ğµ,ğ´]+â€¦+ğœ†ğ‘›ğ‘›![ğµ,[ğµ,[ğµ,â€¦[ğµî„½î„¾î…î…‹î…‹î…‹î…‹î…‹î…‹ğ‘›times,ğ´]]]]â€¦]+â€¦;(16)

if we now set ğµ=ğ‘–ğº we obtain

ğ‘’ğ‘–ğœ†ğºğ´ğ‘’âˆ’ğ‘–ğœ†ğº=ğ‘’ğ‘–ğœ†adğº(ğ´) =ğ´+ğ‘–ğœ†[ğº,ğ´]+â€¦+(ğ‘–ğœ†)ğ‘›ğ‘›![ğº,[ğº,[ğº,â€¦[ğºî„½î„¾î…î…‹î…‹î…‹î…‹î…‹î…‹ğ‘›times,ğ´]]]]â€¦]+â€¦,(17)

where we have used the fact that adğ‘–ğº=ğ‘–adğº, a consequence of the linearity of the bracket [ğº,ğ´] in each of its variables ğ´,ğº. Equation (17) is the desired result. QED.

Note: The technique used here, based on uniqueness of ODEs, is similar in spirit to that used in my answers to several other questions; in particular see this one and this one.

Another Note: A couple of interesting formulas related to the above: [ğµ,ğ‘’ğœ†ğµğ´ğ‘’âˆ’ğœ†ğµ]=ğ‘’ğœ†ğµ[ğµ,ğ´]ğ‘’âˆ’ğœ†ğµ and ğ´=ğ‘’âˆ’ğœ†ğµğ‘’ğœ†adğµ(ğ´)ğ‘’ğœ†ğµ.

Hope this helps. Cheerio,

and as always,

:::